---
layout: post
title:  "Proof 3 (2022/09/25)"
date:   2022-09-25 07:01:36 -0700
categories: jekyll update
mathjax: true
---
<b>Proposition</b>: If $n \in N,$ then $1 + (-1)^n(2n-1)$ is a multiple of $4$.
<hr>

<b>Proof.</b><br>
Suppose $n \in N$. We know $n$ is either odd or even. Consider the following cases:<br>
<b>Case 1:</b> Suppose $n$ is odd. Then $n = 2k + 1$ for some $k \in Z$ and
<div center>
$$
\begin{align*}
1 + (-1)^n(2n-1) &= 1 + (-1)^{(2k+1)}(2(2k+1)-1) \\
&= 1 + (-1)^{(2k+1)}(4k+2-1) \\
&= 1 + -1(4k+1) \\
&= 1 + -4k -1 \\
&= -4k.
\end{align*}
$$
</div>
And we see that $-4k$ is a multiple of 4.
<br>
<b>Case 2:</b> Suppose $n$ is even. Then $n = 2k$ for some $k \in Z$ and
<div center>
$$
\begin{align*}
1 + (-1)^n(2n-1) &= 1 + (-1)^{(2k)}(2(2k)-1) \\
&= 1 + (1)(4k-1) \\
&= 1 + 4k - 1 \\
&= 4k.
\end{align*}
$$
</div>
And we see that $4k$ is also a multiple of 4.$\blacksquare$
<hr>

<b>Refererences:</b>
Book of Proof by Richard Hammack.




