---
layout: post
title:  "[1.6] Remainders (1.6.7)"
date:   2024-11-03 01:01:36 -0700
categories: jekyll update
mathjax: true
---
<!------------------------------------------------------------------------------------>
<div class="peachheaderdiv">
Proposition 1.6.7
</div>
<div class="peachbodydiv">
Given integers \(a\) and \(d\) with \(d \geq 1\), there exists unique integers \(q\) and \(r\) such that 
$$
\begin{align*}
a = qd + r
\end{align*}
$$
where \(0 \leq r < d\). 
</div>
<br>
<b>Proof</b>
<br>
We are given $$a$$ and $$d$$ such that $$d \geq 1$$. <br>
We want to find unique integers $$q$$ and $$r$$ such that $$r < d$$.
<br>
<br>
We have two cases:
<br>
$$a \geq 0$$: If $$d > a$$, then we just take $$q = 0$$ and $$r = a$$.<br>
Otherwise, suppose that $$d \leq a$$. By Induction on a. Assume that for all non-negative integers smaller than $$a$$, we can find such integers. In particular, suppose it holds for $$a - d$$, then there exists integers $$q'$$ and $$r$$ such that
<div> 
$$
\begin{align*}
(a - d) &= q'd + r \quad (\text{where } 0 \leq r < d) \\
a &= q'd + d + r \\
a &= q'(d + 1) + r 
\end{align*}
$$
</div>
And we are done.
<br>
<br>
Case $$a > 0$$: If $$a$$ is divisible by $$d$$, then there exists integer $$q$$ such that $$a = qd$$. So we can set $$r = 0$$ and we are done.
<br>
Otherwise, $$-a > 0$$ so by the first case ($$a \geq 0$$) there exists integers $$q'$$ and $$r'$$ such that $$-a = q'd + r'$$ with $$0 < r' < d$$. So
<div> 
$$
\begin{align*}
-a &= q'd + r' \\
a &= -q'd - r' \\
a &= -q'd - d + d - r' \\
a &= (-q' - 1)d + (d - r') \\
  &= (-q' - 1)d + (d - r').
\end{align*}
$$
</div>
So $$q = (-q' - 1)$$ and $$r = d - r'$$ with $$0 < d - r' < d$$ and we are done.
<br>
<br>
To show that $$q$$ and $$r$$ are unique, suppose for the sake of contradiction that they are not. Therefore suppose that $$a = qd + r = q'd + r'$$ where $$0 \leq r,r' < d$$. Subtracting the equations, we see that
<div> 
$$
\begin{align*}
(q - q')d = r - r'
\end{align*}
$$
</div>
But this means that $$r - r'$$ is divisible by d. However $$|r - r'| \leq \max\{r,r'\} < d$$, so we must have $$|r - r'| = 0$$. This implies that $$(q' - q)d = 0$$ and so $$q' = q$$ as we wanted to show. $$\ \blacksquare$$
<br>
<br>
<hr>
<br>
<!------------------------------------------------------------------------------------>
<h4><b>References</b></h4>
<ul>
<li><a href="https://homepage.divms.uiowa.edu/~goodman/algebrabook.dir/algebrabook.html">Algebra: Abstract and Concrete by Frederick M. Goodman</a></li>
</ul>






















