---
layout: post
title:  "Lecture 13: Cosets"
date:   2025-02-05 01:01:36 -0700
categories: jekyll update
mathjax: true
---
<div class="mintheaderdiv">
Definition 2.4.14
</div>
<div class="mintbodydiv">
Let \(H\) be subgroup of a group \(G\). <br>
\(gH = \{gh \ | \ h \in H\}\) is called a left coset of \(H\) in \(G\). 
<br>
\(Hg = \{hg \ | \ h \in H\}\) is called a right coset of \(H\) in \(G\).
</div>
<br>
<!------------------------------------------------------------------------>
<h4><b>Example</b></h4>
Let $$D_4 = \{e, r, r^2, r^3, j, rj, r^2j, r^3j\}$$. where $$r^4 = e = j^2$$ and $$jr = r^{-1}j$$.
<br> Define the subgroup $$H = \langle j \rangle = \{e, j\}$$. The left cosets are:
<div>
$$
\begin{align*}
eH &= \{e, j\} = jH \\
rH &= \{r, rj\} = rjH \\
r^2H &= \{r^2, r^2j\} = r^2jH \\
r^3H &= \{r^3, r^3j\} = r^3jH \\
\end{align*}
$$
</div>
Notice here that none of the elements overlap between the sets so this gives us a way to partition the set $$G$$ into four pairwise disjoint subsets (We'll prove this next). The right cosets are
<div>
$$
\begin{align*}
He &= \{e, j\} = Hj \\
Hr &= \{r, jr\} = \{e, r^3j\} = Hr^3j \\
Hr^2 &= \{r^2, r^2j\} = Hr^2j \\
Hr^3 &= \{r^3, rj\} = Hrj \\
\end{align*}
$$
</div>
Next we show why these subets must be pairwise disjoint.
<br>
<!------------------------------------------------------------------------>
<div class="peachheaderdiv">
Proposition (2.5.4)
</div>
<div class="peachbodydiv">
Let \(H\) be a subgroup of a group \(G\). If \(X, Y \subseteq G\) are left \(H-\)cosets, then either
<ol>
	<li>\(X \cap Y = \emptyset\).</li>
	<li>\(X = Y\).</li>
</ol>
</div>
<br>
<!------------------------------------------------------------------------>
<b>Proof</b>
<br>
We'll prove that not (1) implies (2) (to prove an or statement). <br>
Suppose that $$g \in X \cap Y$$. We want to show that $$X = Y$$. Since $$X$$ and $$Y$$ are left cosets, then we can write $$X = xH$$ and $$Y = yH$$ for some $$x, y \in G$$. Since $$g \in X \cap Y$$, then we can write $$g = xh_1 = yh_2$$ for some $$h_1, h_2 \in H$$. Observe now that
<div>
$$
\begin{align*}
x &= gh_1^{-1} \\
  &= (yh_2)h_1^{-1} \\
  &= y(h_2h_1^{-1})
\end{align*}
$$
</div>
Likewise
<div>
$$
\begin{align*}
y &= gh_2^{-1} \\
  &= (xh_1)h_2^{-1} \\
  &= x(h_1h_2^{-1})
\end{align*}
$$
</div>
Now, let $$xh \in xH$$, then
<div>
$$
\begin{align*}
xh &= (yh_2h_1^{-1})h \\
   &= y(h_2h_1^{-1}h)
\end{align*}
$$
</div>
But this implies that $$xh \in yH$$. So $$xH \subseteq yH$$. Likewise, let $$yh \in yH$$, then
<div>
$$
\begin{align*}
yh &= (xh_1h_2^{-1})h \\
   &= x(h_1h_2^{-1}h)
\end{align*}
$$
</div>
so $$yh \in xH$$ and $$yH \subseteq xH$$. Therefore $$xH = yH$$. $$\blacksquare$$ 
<br>
<br>
Based on this, we have the following proposition
<br>
<!------------------------------------------------------------------------>
<div class="peachheaderdiv">
Proposition 2.5.3
</div>
<div class="peachbodydiv">
Let \(H\) be a subgroup of a group \(G\), and let \(a\) and \(b\) be
elements of \(G\). The following conditions are equivalent:
<ol type="a">
	<li>\(a \in bH\).</li>
	<li>\(b \in aH\).</li>
	<li>\(aH = bH\).</li>
	<li>\(b^{-1}a \in H\).</li>
	<li>\(a^{-1}b \in H\).</li>
</ol>
</div>
<!------------------------------------------------------------------------>
<br>
<b>Proof (book)</b>
<br>
Suppose $$(a)$$ holds. Let $$a \in bH$$. Then we can write $$a = bh$$. Since $$H$$ is a subgroup, then we know $$h^{-1} \in H$$. So we can write $$b = ah^{-1}$$. But $$ah^{-1}$$ is in $$aH$$ by the definition of a left coset which is what we wanted to show. With similar reason $$(b)$$ also implies $$(a)$$. 
<br>
<br>
For $$(c)$$, we want to show that $$aH \subseteq bH$$ and $$bH \subseteq aH$$. To show that $$bH \subseteq aH$$, we want to show that for any arbitrary element $$x$$ in $$bH$$, that $$x$$ is also in $$aH$$. So consider any $$x \in bH$$. By the definition of a coset, we can write $$x = bh$$ for some $$h \in H$$. Now suppose that $$(b)$$ holds and so we have $$b \in aH$$. This means that we can write $$b = ah_1$$ for some $$h_1 \in H$$. But this means that we can write $$x = bh = ah_1h$$. The product $$h_1h$$ is in $$H$$ because $$H$$ is a subgroup. Furthermore, $$ah_1h$$ must be in $$aH$$ by the definition of a coset. Therefore, $$x = bh \in aH$$ and so $$bH \subseteq aH$$ as we wanted to show. Since $$(b)$$ also implies $$(a)$$ we can use a similar reasoning to show that $$aH \subseteq bH$$.
<br>
<br>
For $$(d)$$ ....
<br>
<br>
<!----------------------------------------------------------------------------->
<h4><b>Lagrange Theorem</b></h4>
Based on what we learned so far, we can now present the most important results
<!------------------------------------------------------------------------>
<div class="peachheaderdiv">
Proposition
</div>
<div class="peachbodydiv">
Let \(H\) be a subgroup of a group \(G\). Then every left \(H-\)coset and right \(H-\)coset has the same size as \(H\).
</div>
<br>
<br>
<div class="peachheaderdiv">
Lagrange Theorem
</div>
<div class="peachbodydiv">
Let \(H\) be a subgroup of a finite group \(G\) (\(|G| = n\). Then \(|H|\) divides \(|G|\).
</div>
<br>
<br>
<div class="peachheaderdiv">
Order Theorem
</div>
<div class="peachbodydiv">
Let \(H\) be a subgroup of a finite group \(G\). If (\(|G| = n\). Then for any \(g \in G\), \(o(g) = |\langle g \rangle|\) divides \(|G|\).
</div>





<br>
<hr>
<br>
<!----------------------------------------------------------------------------->
<h4><b>References</b></h4>
<ul>
	<li>MATH417 by Charles Rezk</li>
	<li><a href="https://homepage.divms.uiowa.edu/~goodman/algebrabook.dir/algebrabook.html">Algebra: Abstract and Concrete by Frederick M. Goodman</a></li>
</ul>






















