---
layout: post
title:  "Extra Proofs / Study Notes"
date:   2025-02-14 01:01:36 -0700
categories: jekyll update
mathjax: true
---
<h4><b>Example 1</b></h4>
<!----------------------------------------------------------------------------->
<div class="peachheaderdiv">
Proposition
</div>
<div class="peachbodydiv">
Suppose \((x,y) \in G_1 \times G_2\) and that the order of the elements are \(|x| = r\) and \(|y| = s\). Then the order of \((x,y)\) is \(lcm(r,s)\)
</div>
<br>
<!----------------------------------------------------------------------------->
<b>Proof</b>
<br>
Let $$l = lcm(r,s)$$. Then, $$l = ra = sb$$ for some $$r, b \in \mathbf{Z}$$. Observe that
<div>
	$$
	\begin{align*}
	(x,y)^{l} &= (x^l, y^l) = (x^{ra}, y^{sb}) = (e_1, e_2)
	\end{align*}
	$$
</div>
From this we see that the order of $$(x,y)$$ must divide $$l$$. If we let $$l' = |(x,y)|$$, then  $$l' \ | \ l$$. Now, observe that
<div>
	$$
	\begin{align*}
	(x,y)^{l'} &= (x^{l'}, y^{l'}) = (e_1, e_2)
	\end{align*}
	$$
</div>
But since $$|x| = r$$ and $$|y| = s$$, then $$r \ | \ l'$$ and $$s \ | \ l'$$. But this means that $$lcm(r,s) = l \ | \ l'$$. Since $$l' \ | \ l$$ and $$l \ | \ l'$$, then $$l = l'$$ as we wanted to show.
<br>
<br>
<hr>
<br>
<!----------------------------------------------------------------------------->
<h4><b>Example 2</b></h4>
<!----------------------------------------------------------------------------->
<div class="peachheaderdiv">
Proposition
</div>
<div class="peachbodydiv">
\(\mathbf{Z}_m \times \mathbf{Z}_n \cong \mathbf{Z}_{mn}\) if and only if \(gcd(m,n) = 1\)
</div>
<br>
This says if you take the product of two cyclic groups, then their product is cyclic if and only if $$m$$ and $$n$$ are relatively prime.
<br>
<br>
<!----------------------------------------------------------------------------->
<b>Proof</b>
<br>
$$\longrightarrow:$$ Suppose $$\mathbf{Z}_m \times \mathbf{Z}_n \cong \mathbf{Z}_{mn}$$. Suppose for the sake of contradiction that $$gcd(m,n) = d > 1$$. Now, take an arbitrary element $$(a,b) \in \mathbf{Z}_m \times \mathbf{Z}_n$$. Add $$(a,b)+...+(a,b)$$ $$\frac{mn}{d}$$ times. We will see that 
<div>
	$$
	\begin{align*}
	(a\frac{mn}{d},b\frac{mn}{d}) &= (a\frac{n}{d}m,b\frac{m}{d}n) \\
	                              &= ([0]_m, [0]_n)
	\end{align*}
	$$
</div>
Notice here that both $$\frac{n}{d}$$ and $$\frac{m}{d}$$ are whole numbers since $$d$$ is a divisor of both $$m$$ and $$n$$. So the first entry is a multiple of $$m$$ while the second entry is a multiple of $$n$$. This implies that the order of $$(a,b) \leq \frac{mn}{d} < mn$$. So the order of any element $$(a,b) \in \mathbf{Z}_m \times \mathbf{Z}_n$$ is strictly less than $$mn$$. This means that no element of $$\mathbf{Z}_m \times \mathbf{Z}_n$$ can be a generator of the group. So $$\mathbf{Z}_m \times \mathbf{Z}_n$$ is not cyclic. This is a contradiction because $$\mathbf{Z}_m \times \mathbf{Z}_n$$ isomorphic to $$\mathbf{Z}_{mn}$$ and so it is cyclic. 
<br>
<br>
$$\longleftarrow:$$ Now suppose that $$gcd(m,n) = 1$$. We want to show that $$\mathbf{Z}_m \times \mathbf{Z}_n$$ is isomorphic to $$\mathbf{Z}_{mn}$$. Notice that the order of the element 1 has order $$m$$ in $$\mathbf{Z}_m$$ and the order of the element 1 has order $$n$$ in $$\mathbf{Z}_n$$. This tells us that the order of $$(1,1) = lcm(m,n) \frac{mn}{gcd(m,n)} \frac{mn}{1} = mn$$. So $$(1,1)$$ has order $$mn$$ which means it generates the group. So it must be cyclic. So $$\mathbf{Z}_m \times \mathbf{Z}_n = \langle (1,1) \rangle$$. We know all cyclic groups that have the same order are isomorphic. So $$\mathbf{Z}_m \times \mathbf{Z}_n \cong \mathbf{Z}_{mn}$$.
<br>
<br>
<hr>
<br>
<!----------------------------------------------------------------------------->
<h4><b>Example 3</b></h4>
Let $$Q_8 = \{1, -1, i, i, j, -j, k, -k\}$$ be a group. We have the identities:
<div>
	$$
	\begin{align*}
	i^2 = j^2 = k^2 = -1, \quad ij = k, \quad ji = -k, \quad ijk = -1
	\end{align*}
	$$
</div>
<br>
$$ij = k$$ is going in a clockwise direction while $$ji = -k$$ is going in a counter clockwise direction.
TODO: Group diagram.
<br>
<br>
There are three cyclic subgroups of order 4: $$\langle i \rangle$$, $$\langle j \rangle$$ and $$\langle k \rangle$$. There is one cyclic group of order 2: $$\langle -1 \rangle$$. Note that $$\langle i \rangle = \{1, i, -1, -i\}$$. 
<br>
<br>
Let's find the cosets of $$\langle i \rangle$$ in $$Q_8$$. 
<div>
	$$
	\begin{align*}
	j\langle i \rangle &= j\{1, i, -1, -i\} = \{j, -k, -j, k\} \\
	\langle i \rangle j &= \{1, i, -1, -i\}j = \{j, k, -j, -k\}
	\end{align*}
	$$
</div>
Note that $$Q_8$$ is generated by two elements $$\langle i, j \rangle$$ (easy to check). Therefore, since $$j\langle i \rangle = \langle i \rangle j$$ and we checked all the generators of the group, then $$\langle i \rangle$$ is a normal subgroup.
<br>
<br>
Let's study the quotient group $$Q_8 / \langle i \rangle$$. We know that it must contain two elements (By Lagrange's Theorem).
<div>
	$$
	\begin{align*}
	Q_8 / \langle i \rangle = \{\langle i \rangle, j \langle i \rangle\}
	\end{align*}
	$$
</div>
<br>
<br>
Recall, that we defined the multiplication of cosets by $$(xN)(yN)=(xy)N$$. Since we have two elements, observe that $$\langle i \rangle \langle i \rangle = \langle i \rangle$$. Multiply $$j \langle i \rangle$$ by $$\langle i \rangle$$ is just $$j \langle i \rangle$$. Remember that $$\langle i \rangle$$ acts as the identity element/coset here. So the only interesting product is $$(j\langle i \rangle) (j\langle i \rangle)$$ [TODO: add a table]
<div>
	$$
	\begin{align*}
	(j\langle i \rangle) (j\langle i \rangle) &= j^2 \langle i \rangle = -\langle i \rangle = \langle i \rangle. 
	\end{align*}
	$$
</div>
This multiplication table looks like the multiplication table of $$\mathbf{Z}_2$$. In fact $$Q_8 / \langle i \rangle \cong \mathbf{Z}_2$$.
<br>
<br>
<hr>
<br>
<!----------------------------------------------------------------------------->
<h4><b>Example 4</b></h4>
Taking $$Q_8$$ from before, let's look at at the cyclic group generated by $$\langle -1 \rangle$$.
<div>
	$$
	\begin{align*}
	\langle -1 \rangle &= \{-1, 1\} 
	\end{align*}
	$$
</div>
$$\langle -1 \rangle$$ is a normal subgroup (easy check, every element in the subgroup commutes with all elements in $$Q_8$$). So we now look at the quotient structure. (the cosets of $$\langle -1 \rangle$$ in $$Q_8$$)
<div>
	$$
	\begin{align*}
	i \langle -1 \rangle &= \{-i, i\} \\
	j \langle -1 \rangle &= \{-j, j\} \\
	k \langle -1 \rangle &= \{-k, k\} \\
	Q_8 / \langle -1 \rangle &= \{i \langle -1 \rangle , i \langle -1 \rangle, j \langle -1 \rangle, k \langle -1 \rangle \}
	\end{align*}
	$$
</div>
Let's calculate the order of each element. For example, $$(i \langle -1 \rangle)^2 = -1\langle -1 \rangle = \langle -1 \rangle$$. So $$o(i\langle -1 \rangle) = 2$$. In fact, we also have $$o(j\langle -1 \rangle) = 2$$ and $$o(k\langle -1 \rangle) = 2$$. This isn't cyclic so this group must be isomorphic to the non-cyclic group of order 4. So it's isomorphic to $$\mathbf{Z}_2 \times \mathbf{Z}_2$$. 
<br>
<br>
<hr>
<br>
<!----------------------------------------------------------------------------->
<h4><b>Example 5</b></h4>
Suppose that we are given
<div>
	$$
	\begin{align*}
	\phi: \mathbf{Z} &\rightarrow \mathbf{Z}_n \\
	                 &\phi(m) = [m] = \{k \in \mathbf{Z} \ | \ k \equiv m (\bmod n)\}
	\end{align*}
	$$
</div>
We want to show that $$\phi(m)$$ is surjective. This is because for all $$0 \leq m \leq m - 1$$, $$\phi(m) = [m]$$ So we are able to hit every value of $$m$$. It is also a homomorphism. since 
<div>
	$$
	\begin{align*}
	\phi(m_1 + m_2) = [m_1 + m_2] = [m_1] + [m_2] = \phi(m_1) + \phi(m_2)
	\end{align*}
	$$
</div>
The kernel of $$\phi$$ is 
<div>
	$$
	\begin{align*}
	\ker(\phi) &= \{ m \in \mathbf{Z} \ | \ [m] = [0]\} \\
	           &= \{0, \pm n, \pm 2n,....\} = n\mathbf{Z}
	\end{align*}
	$$
</div>
So now we have $$\ker(\phi) = n\mathbf{Z}$$. We know that it is normal. We also showed that $$\phi$$ is a surjective homomorphism. Therefore, by the Isomorphism Theorem, $$\mathbf{Z}/n\mathbf{Z} \cong \mathbf{Z}_n$$.
<br>
<br>
<hr>
<br>
<!----------------------------------------------------------------------------->
<h4><b>Example 6</b></h4>
Next, let's take 
<div>
	$$
	\begin{align*}
	\phi: \mathbf{Z}_4 &\rightarrow \mathbf{Z}_2 \\
	        &\phi([m]_4) = [m]_2 
	\end{align*}
	$$
</div>
Here, it is not obvious this is well-defined. So let's check that it is. Suppose that $$[m_1]_4 = [m_2]_4$$. We want to show that $$\phi([m_1]_4) = \phi([m_2]_4)$$. Observe that
<div>
	$$
	\begin{align*}
	[m_1]_4 &= [m_2]_4 \\
	[m_1]_4 - [m_2]_4 &= [0]_4 \\
	[m_1 - m_2]_4 &= [0]_4 \\
	m_1-m_2 &\equiv 0 \bmod 4
	\end{align*}
	$$
</div>
This says that $$m_1 - m_2$$ must be a multiple of 4 so $$m_1 - m_2 = 4k = 2(2k)$$ for some $$k \in \mathbf{Z}$$. So $$m_1 - m_2$$ is also a multiple of 2. Therefore, $$m_1-m_2 \equiv 0 \bmod 2$$ and so $$[m_1]_2 = [m_2]_2$$.
<br>
<br>
$$\phi$$ is also a homomorphism. since 
<div>
	$$
	\begin{align*}
	\phi([m_1]_4 + [m_2]_4) = \phi([m_1 + m_2]_4) = [m_1 + m_2]_2 = [m_1]_2 + [m_2]_2 = \phi(m_1) + \phi(m_2).
	\end{align*}
	$$
</div>
Next we want to show that $$\phi$$ is surjective. Notice that there are two values in the target domain. $$[0]_2$$ and $$[1]_2$$. Also note that $$\phi([0]_4) = [0]_2$$ and $$\phi([1]_4) = [1]_2$$ so it is surjective.
<br>
<br>
The kernel of $$\phi$$ is 
<div>
	$$
	\begin{align*}
	\ker(\phi) &= \{ [m]_4 \in \mathbf{Z}_4 \ | \ \phi([m]_4) = [0]_2\} \\
	           &= \{ [m]_4 \in \mathbf{Z}_4 \ | \ [m]_2 = [0]_2\} \\
			   &= \{ [0]_4, [2]_4 \} = \langle [2]_4 \rangle = 2\mathbf{Z}_4 \\
	\end{align*}
	$$
</div>
So now we have $$\ker(\phi) = \langle [2]_4 \rangle$$. We know that it is normal. We also showed that $$\phi$$ is a surjective homomorphism. Therefore, by the Isomorphism Theorem, $$\mathbf{Z}_4/\langle [2]_4 \rangle \cong \mathbf{Z}_2$$.
<br>
<br>
<hr>
<br>
<!----------------------------------------------------------------------------->
<h4><b>Example 7</b></h4>
Next, let's take 
<div>
	$$
	\begin{align*}
	\phi: \mathbf{Z}_6 &\rightarrow \mathbf{Z}_{15}
	\end{align*}
	$$
</div>
We need to figure out a homomorphism. First recall that for any element, $$|\phi(x)| \ | \ |x|$$. Let's list the order of the elements in $$\mathbf{Z}_{15}$$. Notice here that $$\mathbf{Z}_{15}$$ is a cyclic group (with addition) so the order of any element $$g + a$$ is going to be $$\frac{15}{gcd(a,15)}$$
<div>
	$$
	\begin{align*}
	&o(1): [0]_{15} \\
	&o(3): [5]_{15}, [10]_{15} \\
	&o(5): [3]_{15}, [6]_{15}, [9]_{15}, [12]_{15} \\
	&o(15): [1]_{15}, [2]_{15}, [4]_{15}, [7]_{15}, [11]_{15}, [13]_{15}, [14]_{15} \\
	\end{align*}
	$$
</div>
So now let's pick $$[1]_{6}$$. It is a generator for $$\mathbf{Z}_{6}$$. We know that $$\phi([1]_6)$$ must divide the order of the element itself so $$|[1]_6| = 6$$. So that tells us that $$|\phi([1]_6)|$$ must be either 1,2,3 or 6. 2 and 6 are not possibilities so we don't have any elements of that order in $$\mathbf{Z}_{15}$$. So it's either 1 or 3.
<br>
<br>
Case 1: Suppose we pick some element of order 1. That means that $$\phi([1]_6) = 1$$. This implies that $$\phi([1]_6) = [0]_{15}$$. Since it's a generator, then $$\ker(\phi) = \mathbf{Z}_6$$. And $$Im(\phi) = \{[0]_{15}\}$$. This gives us $$\mathbf{Z}_6/\mathbf{Z}_6 = \{[0]_{15}\} \leq \mathbf{Z}_{15}$$. So it's pretty boring.
<br>
<br>
Case 2: Suppose we pick some element of order 3 so $$|\phi([1]_6)| = 3$$. So let $$\phi([1]_6) = [5]_{15}$$. Based on this, where will $$[2]_6$$ will go? Remember that we want $$\phi$$ to be a homomorphism. This means that we want this to be true. That $$\phi([2]_6) = \phi([1 + 1]_6) = \phi([1]_6) + \phi([1]_6) = [5]_{15} + [5_{15} = [10]_{15}$$. So we want to pick $$[10]_{15}$$ for $$[2]_6$$. Based on this, the elements will get mapped to 
<div>
	$$
	\begin{align*}
	[0]_6 &\rightarrow [0]_{15} \\
	[1]_6 &\rightarrow [5]_{15} \\
	[2]_6 &\rightarrow [10]_{15} \\
	[3]_6 &\rightarrow [0]_{15} \\
	[4]_6 &\rightarrow [5]_{15} \\
	[5]_6 &\rightarrow [10]_{15}.
	\end{align*}
	$$
</div>
So the image of our homomorphism is 
<div>
	$$
	\begin{align*}
	Im(\phi) = \{[0]_{15}, [5]_{15}, [10]_{15}\} = \langle [5]_{15} \rangle \cong \mathbf{Z}_3
	\end{align*}
	$$
</div>
The last statement is because all cyclic groups of order 3 are isomorphic to $$\mathbf{Z}_3$$. The kernel of $$\phi$$ is 
<div>
	$$
	\begin{align*}
	\ker(\phi) &= \{ [m]_6 \in \mathbf{Z}_6 \ | \ \phi([m]_6) = [0]_{15}\} \\
			   &= \{ [0]_6, [3]_{6} \} = \langle [3]_6 \rangle \cong \mathbf{Z}_2\\
	\end{align*}
	$$
</div>
By the Isomorphism Theorem, $$\mathbf{Z}_{6}/\langle [3]_6 \rangle \cong \langle [5]_{15} \rangle \cong \mathbf{Z}_3$$.
<br>
<br>
<hr>
<br>
<!----------------------------------------------------------------------------->
<h4><b>References</b></h4>
<ul>
	<li><a href="https://www.youtube.com/watch?v=ako25Pghxa8">The order of an element in a direct group is the lcm of both elements orders</a></li>
	<li><a href="https://www.youtube.com/watch?v=BE8lhcGfSiI&list=PL22w63XsKjqwN7sHsEiy0yqkcjQfXAuVb&index=12">Isomorphism Examples</a></li>
</ul>






















