---
layout: post
title:  "[2.5] Cosets and Lagrangeâ€™s Theorem"
date:   2025-01-01 01:01:36 -0700
categories: jekyll update
mathjax: true
---
<div class="mintheaderdiv">
Definition 2.4.14
</div>
<div class="mintbodydiv">
Let \(H\) be subgroup of a group \(G\). A subset of the form
\(gH\), where \(g \in G\), is called a left coset of \(H\) in \(G\). A subset of the form
\(Hg\), where \(g \in G\), is called a right coset of \(H\) in \(G\).
</div>
<br>
<!------------------------------------------------------------------------>
<h4><b>Example 1</b></h4>
Consider H = $$\{e , (1,2)\} \subseteq S_3$$. We know $$S_3$$ has six elements. Let $$\pi \in S_3$$ and compute $$\pi H = \{ \pi \sigma \ : \ \sigma \in H \}$$. So
<div>
$$
\begin{align*}
S_3 = \{ e, \begin{pmatrix}1 & 2 \end{pmatrix}, \begin{pmatrix}1 & 3 \end{pmatrix}, \begin{pmatrix}2 & 3 \end{pmatrix}, \begin{pmatrix}1 & 2 & 3 \end{pmatrix}, \begin{pmatrix}1 & 3 & 2 \end{pmatrix} 
\}
\end{align*}
$$
</div>
For example $$ \begin{pmatrix}1 & 3 \end{pmatrix} H$$ is
<div>
$$
\begin{align*}
\begin{pmatrix}1 & 3 \end{pmatrix} H &= \{ \begin{pmatrix}1 & 3 \end{pmatrix}e, \begin{pmatrix}1 & 3 \end{pmatrix}  \begin{pmatrix}1 & 2 \end{pmatrix} \} \\
&= \{ \begin{pmatrix}1 & 3 \end{pmatrix}, \begin{pmatrix} 1 & 2 & 3 \end{pmatrix} \}
\end{align*}
$$
</div>
This is because if we let $$f = (1 \quad 3)$$ and $$g = (1 \quad 2)$$, then $$f \circ g$$ results in $$f(g(1)) = f(2) = 2$$. So 1 gets mapped to 2. Similarly $$f(g(2)) = f(1) = 3$$. So 2 gets mapped to 3 and $$f(g(3)) = f(3) = 1$$ so 3 gets mapped to 1. Writing this in cycle notation means $$1 \rightarrow 2, 2 \rightarrow 3, 3 \rightarrow 1$$ or $$(1 \quad 2 \quad 3)$$. 
<div>
$$
\begin{align*}
eH &= (1 \quad 2) H = H \\
\begin{pmatrix}1 & 3 \end{pmatrix} H &= (1 \quad 2 \quad 3)H = \{ \begin{pmatrix}1 & 3 \end{pmatrix}, \begin{pmatrix}1 & 2 & 3 \end{pmatrix} \} \\
\begin{pmatrix}2 & 3 \end{pmatrix} H &= (1 \quad 3 \quad 2)H = \{ \begin{pmatrix}2 & 3 \end{pmatrix}, \begin{pmatrix}1 & 3 & 2 \end{pmatrix} \} \\
\end{align*}
$$
</div>
<br>
<hr>
<br>
<!------------------------------------------------------------------------>
<h4><b>Example 2</b></h4>
Suppose $$G = (\mathbf{Z}_4, +)$$ and $$H = \{0, 2\}. Then we have the following cosests
<div>
$$
\begin{align*}
H+0 &= \{0,2\} \\
H+1 &= \{1,3\} \\
H+2 &= \{2,0\} \\
H+3 &= \{3,1\}
\end{align*}
$$
</div>
We can see here that we have two distinct right cosets. Moreover, the cosets are disjoint and partition the group. Next, we'll formalize these properties about cosets!
<br>
<br>
<!------------------------------------------------------------------------>
<div class="peachheaderdiv">
Proposition 2.5.3
</div>
<div class="peachbodydiv">
Let \(H\) be a subgroup of a group \(G\), and let \(a\) and \(b\) be
elements of \(G\). The following conditions are equivalent:
<ol type="a">
	<li>\(a \in bH\).</li>
	<li>\(b \in aH\).</li>
	<li>\(aH = bH\).</li>
	<li>\(b^{-1}a \in H\).</li>
	<li>\(a^{-1}b \in H\).</li>
</ol>
</div>
<!------------------------------------------------------------------------>
<br>
<b>Proof</b>
<br>
Suppose $$(a)$$ holds. Let $$a \in bH$$. Then there exists some $$h \in H$$ such that $$a = bh$$. Since $$H$$ is a subgroup, then we know $$h^{-1} \in H$$. So we can write $$b = ah^{-1}$$. But $$ah^{-1}$$ is in $$aH$$ by the definition of a left coset which is what we wanted to show. With similar reason $$(b)$$ also implies $$(a)$$. 
<br>
<br>
For $$(c)$$, we want to show that $$aH \subseteq bH$$ and $$bH \subseteq aH$$. To show that $$bH \subseteq aH$$, we want to show that for any arbitrary element $$x$$ in $$bH$$, that $$x$$ is also in $$aH$$. So consider any $$x \in bH$$. By the definition of a coset, we can write $$x = bh$$ for some $$h \in H$$. Now suppose that $$(b)$$ holds and so we have $$b \in aH$$. This means that we can write $$b = ah_1$$ for some $$h_1 \in H$$. But this means that we can write $$x = bh = ah_1h$$. The product $$h_1h$$ is in $$H$$ because $$H$$ is a subgroup. Furthermore, $$ah_1h$$ must be in $$aH$$ by the definition of a coset. Therefore, $$x = bh \in aH$$ and so $$bH \subseteq aH$$ as we wanted to show. Since $$(b)$$ also implies $$(a)$$ we can use a similar reasoning to show that $$aH \subseteq bH$$.
<br>
<br>
For $$(d)$$ ....
<br>
<br>
<!------------------------------------------------------------------------>
<div class="peachheaderdiv">
Proposition 2.5.4
</div>
<div class="peachbodydiv">
Let \(H\) be a subgroup of a group \(G\).
<ol type="a">
	<li>Let \(a\) and \(b\) be elements of \(G\). Either \(aH = bH\) or \(aH \cap bH = \emptyset\)</li>
	<li>Each left coset \(aH\) is nonempty and the union of left cosets is \(G\).</li>
</ol>
</div>
<!------------------------------------------------------------------------>
<br>
<b>Proof</b>
<br>
For $$(a)$$, Suppose $$aH \cap bH \neq \emptyset$$ and let $$c \in aH \cap bH$$. Since $$c \in aH$$, then $$aH = cH$$ by Proposition 2.5.3. Similarly since $$c \in bH$$, then $$bH = cH$$. Therefore, $$aH = bH$$.
<br>
<br>
For $$(b)$$, $$aH$$ is nonempty since $$H$$ is a subgroup and can't be empty. Furthermore, for each element $$g \in G$$, $$g \in gH$$. By $$(a)$$ then the union of all the left cosets must be $$G$$.
<br>
<br>
<!------------------------------------------------------------------------>
<div class="peachheaderdiv">
Proposition 2.5.5
</div>
<div class="peachbodydiv">
Let \(H\) be a subgroup of a group \(G\) and let \(a\) and \(b\) be
elements of \(G\). Then \(x \longmapsto ba^{-1}\) is a bijection between \(aH\) and \(bH\).
</div>
<!------------------------------------------------------------------------>
<br>
<b>Proof</b>
Let $$f : aH \rightarrow bH$$ where $$f(x) = ba^{-1}x$$. We want to show that $$f$$ is a bijection by showing that it's one-to-one and onto. Suppose $$a_1, a_2 \in aH$$ then we can write $$a_1 = ah_1$$ and $$a_2 = ah_2$$ for some $$h_1, h_2 \in H$$. Moreover, suppose that $$f(a_1) = f(a_2)$$. Observe that
<div>
$$
\begin{align*}
ba^{-1}a_1 &= ba^{-1}a_2 \\
b^{-1}ba^{-1}a_1 &= b^{-1}ba^{-1}a_2 \quad \text{($G$ is a group so the inverse exists)} \\
aa^{-1}a_1 &= aa^{-1}a_2 \\
a_1 &= a_2 \\
\end{align*}
$$
</div>
From this we see that $$f$$ is one-to-one or injective. To see that it's surjective, we need to show that for any element $$y \in bH$$, that there exists an element $$x \in aH$$ such that $$f(x) = y$$. Since $$y \in bH$$, then we can write $$y = bh$$ for some $$h \in H$$. Now, let $$x = ah \in aH$$ and observe that
<div>
$$
\begin{align*}
f(x) &= ba^{-1}x \\
     &= ba^{-1}(ah) \\
	 &= b(a^{-1}ah) \\
	 &= bh = y.
\end{align*}
$$
</div>
$$ah$$ is in $$aH$$ by definition. Therefore $$f$$ is surjective. From this we see that $$f$$ is a bijection from $$aH$$ to $$bH$$. $$\ \blacksquare$$
<br>
<br>
<!------------------------------------------------------------------------>
<div class="yellowheaderdiv">
Theorem 2.5.6 (Lagrange's Theorem)
</div>
<div class="yellowbodydiv">
Let \(G\) be a finite group and \(H\) a subgroup. Then the cardinality of \(H\) divides the cardinality of \(G\), and the quotient \(\frac{|G|}{|H|}\) is the number of left cosets of \(H\) in \(G\).
</div>
<!------------------------------------------------------------------------>
<br>
<b>Proof</b>







<br>
<br>
<br>
<hr>
<br>
<!------------------------------------------------------------------------>
<h4><b>References</b></h4>
<ul>
<li><a href="https://homepage.divms.uiowa.edu/~goodman/algebrabook.dir/algebrabook.html">Algebra: Abstract and Concrete by Frederick M. Goodman</a></li>
<li><a href="https://www.youtube.com/watch?v=kthl-MhIf4s&list=PLztBpqftvzxVvdVmBMSM4PVeOsE5w1NnN&index=22">Wrath of Math Youtube Channel</a></li>
</ul>






















