---
layout: post
title:  "Lecture 06: Least Common Multiple"
date:   2025-01-29 01:01:36 -0700
categories: jekyll update
mathjax: true
---
<div class="mintheaderdiv">
Definition
</div>
<div class="mintbodydiv">
A least common multiple (LCM) is \(m \in \mathbf{Z_{\geq 0}}\) such that:
<ol type="a">
	<li>\(a \ | \ m\) and \(b \ | \ m\)</li>
	<li>If \(n \in \mathbb{Z}\), \(a \ | \ n\) and \(b \ | \ n\), then \(m \ | \ n\).</li>
</ol>
</div>
<!------------------------------------------------------------------------>
<br>
<br>
In fact the LCM is unique if it exists. To prove it's existence we'll need the following definition
<br>
<br>
<!------------------------------------------------------------------------>
<div class="mintheaderdiv">
Definition (Well Ordering Principle)
</div>
<div class="mintbodydiv">
A non-empty subset of \(\mathbb{N}\) has a smallest element
</div>
<!------------------------------------------------------------------------>
<br>
<br>
Next, we'll prove the existence of the LCM.
<br>
<br>
<!------------------------------------------------------------------------>
<div class="peachheaderdiv">
Proposition
</div>
<div class="peachbodydiv">
The LCM always exists
</div>
<!------------------------------------------------------------------------>
<br>
<b>Proof</b>
<br>
Let $$a, b \in \mathbb{Z}$$. Let $$J = \mathbb{Z}a \cap \mathbb{Z}b$$. We want to show that $$J$$ itself is a set of multiples so we can write $$J = \mathbb{Z}m$$ for some $$m \in \mathbb{Z}_{\geq 0}$$. This means that $$m$$ must be the LCM of $$a$$ and $$b$$ by definition. [Why? If $$J = \mathbb{Z}m$$, then $$m$$ is the least element in $$J$$, all the other elements are multiples of $$m$$. We have $$a \ | \ m$$ and $$b \ | \ m$$ because $$J$$ also contains common multiples of $$a$$ and $$b$$. And for any $$n \in \mathbb{Z}$$, if $$a \ | \ n$$ and $$b \ | \ n$$, then $$m \ | \ n$$. This is true because $$m$$ is the smallest of all these common multiples.] We will use division by remainder to prove this!
<br>
<br>
Observe that $$J$$ is closed under addition and subtraction. So if $$c, d \in J$$, then any integer combination of $$c$$ and $$d$$ will be in $$J$$. So for any $$m, n \in \mathbb{Z}$$,  $$cm + dn \in J$$.
<br>
<br>
We have two cases:
<br>
Case 1: If either $$a = 0$$ or $$b = 0$$, then $$J = \{0\} = \mathbb{Z}0$$.
<br>
<br>
Case 2: If $$ a \neq 0$$ and $$b \neq 0$$, then $$J$$ is the set of common multiples of $$\mathbb{Z}a$$ and $$\mathbb{Z}b$$. Consider $$J \cap \mathbb{N}$$. This is the set of positive common multiples. This set is not empty because it will at least include $$|ab|$$. So $$J \cap \mathbb{N}$$ is a non-empty subset of $$\mathbb{N}$$. By the well-ordering principle, there is a smallest number in $$J \cap \mathbb{N}$$. Let $$m \in J \cap \mathbb{N}$$ be the smallest common multiple. (so we're setting $$m$$ to be the smallest positive common multiple of $$\mathbb{Z}a$$ and $$\mathbb{Z}b$$)
<br>
<br>
We claim that $$J = \mathbb{Z}m$$ (the set of multiples of $$m$$). We will show this by proving that $$J \subseteq \mathbb{Z}m$$ and that $$\mathbb{Z}m \subseteq J$$. 
<br>
<br>
$$\mathbb{Z}m \subseteq J$$: This is true since $$m \in J$$ and we showed earlier that $$m$$ is closed under addition and subtraction so any multiple of $$m$$ is also in $$J$$ and therefore $$\mathbb{Z}m \subseteq J$$.
<br>
<br>
$$J \subseteq \mathbb{Z}m$$: Suppose $$x \in J = \mathbb{Z}a \cap \mathbb{Z}b$$. Consider what happens when we divide $$x$$ by $$m$$. We can write $$x = qm + r$$. with $$q, r \in \mathbb{Z}$$ and $$0 \leq r < m$$. Re-write the equation as
<div>
$$
\begin{align*}
r = x - qm.
\end{align*}
$$
</div>
Observe now that $$x \in J$$ by assumption. $$qm$$ is a multiple of $$m$$ so it's in $$J$$. So their difference is also in $$J$$ which means that $$r \in J$$. If $$r = 0$$, $$x = qm \in \mathbb{Z}m$$ and we're done. If $$r \neq 0$$, then $$r \in J$$, then $$r \in J \cap \mathbb{N}$$ but also $$r < m$$. But that's a contradiction because $$m$$ is the smallest element in $$J \cap \mathbb{N}$$ and so this case doesn't happen. So $$J = \mathbb{Z}m$$ as desired. $$\ \blacksquare$$.
<hr>

<!------------------------------------------------------------------------>
<h3>Consequences of the LCM</h3>
The next few propositions are some consequences of the LCM.
<br>
<br>
<div class="peachheaderdiv">
Proposition
</div>
<div class="peachbodydiv">
If \(d = gcd(a,b) = 1\), then \(m = lcm(a,b) = ab\)
</div>
<!------------------------------------------------------------------------>
<br>
<b>Proof</b>
<br>
We are given that $$d = gcd(a,b) = 1$$. This means that $$a$$ and $$b$$ are relatively prime. Condition 1 is true since $$a \ | \ ab$$ and $$b \ | \ ab$$. For condition two of the LCM definition, let $$n \in \mathbb{Z}$$ such that $$a \ | \ n$$ and $$b \ | \ n$$. By the proposition from lecture 5, $$ab \ | \ n$$. (Proposition: If $$a$$ and $$b$$ are relatively prime, then if $$a \ | \ n$$ and $$b \ | \ n$$, then $$ab \ | \ n$$). $$\ \blacksquare$$
<br>
<br>
<!------------------------------------------------------------------------>
<div class="peachheaderdiv">
Proposition
</div>
<div class="peachbodydiv">
Let \(e\) be a common divisor of \(a\) and \(b\) so \(e \ | \ a\) and \(e \ | \ b\). Then \(lcm(\frac{a}{e}, \frac{b}{e}) = \frac{1}{e} lcm(a,b)\). 
</div>
<!------------------------------------------------------------------------>
<br>
<b>Proof</b>
<br>
[TODO] $$x$$ is a common divisor of $$\frac{a}{e}$$ and $$\frac{b}{e}$$ if and only if $$xe$$ is a common divisor of $$a$$ and $$b$$. 
<br>
<br>
<!------------------------------------------------------------------------>
<div class="peachheaderdiv">
Proposition
</div>
<div class="peachbodydiv">
If \(a, b \in \mathbb{N}\), \(d = gcd(a,b)\) and \(m = lcm(a,b)\), then \(m = \frac{ab}{d}\)
</div>
<!------------------------------------------------------------------------>
<br>
<b>Proof</b>
<br>
We need the previous two propositions
<ol>
	<li>If \(d = 1\), then \(m = lcm(a,b) = ab\)</li>
	<li>If \(e \ | \ a\) and \(e \ | \ b\), then \(lcm(\frac{a}{e}, \frac{b}{e}) = \frac{1}{e} lcm(a,b)\)</li>
</ol>
If we divide both $$a$$ and $$b$$ by $$d$$, their gcd will become 1 so $$gcd(\frac{a}{d}, \frac{b}{d}) = 1$$. Since the gcd is 1, then $$lcm(\frac{a}{d}, \frac{b}{d}) = \frac{b}{d}\frac{a}{d}$$ by part $$(1)$$. So now let $$e = d$$, so by $$(2)$$, 
<div>
$$
\begin{align*}
\frac{1}{d} lcm(a, b) &= lcm(\frac{a}{d}, \frac{b}{d}) \\
\frac{m}{d}  &= \frac{b}{d}\frac{a}{d} \\
m &= \frac{ab}{d} \\
\end{align*}
$$
</div>
<hr>

<!------------------------------------------------------------------------>
<h3>Pairwise Relatively Prime</h3>
<br>
<div class="mintheaderdiv">
Definition
</div>
<div class="mintbodydiv">
\(a_1,...,a_k \in \mathbb{Z}\) are pairwise relatively prime if \(gcd(a_i,a_j) = 1\) for all \(1 \leq i,j \leq k, i \neq j\)
</div>
<br>
Some facts based this:
<br>
<br>
<!------------------------------------------------------------------------>
<div class="yellowheaderdiv">
Lemma
</div>
<div class="yellowbodydiv">
If \(a_1,...,a_k \in \mathbb{Z}\) are pairwise relatively prime, then \(a_k,b = a_1,...,a_{k-1}\) are relatively prime so \(gcd(a_k,b) = 1\). 
</div>
<!------------------------------------------------------------------------>
<br>
<b>Proof</b>
<br>
Suppose for the sake of contradiction that $$a_k$$ and $$b$$ are not relatively prime so they have a common divisor. Let $$p$$ be a prime that is a common divisor of $$a_k$$ and $$b$$. So $$p \ | \ b$$ which means that $$p \ | \ a_1a_2...a_{k-1}$$. But since $$p$$ is prime, then by the proposition from the previous lecture, $$p$$ must divide one of the factors in $$a_1a_2...a_{k-1}$$. Let $$p$$ divide $$a_i$$ for some $$1 \leq i \leq k - 1$$. However $$p \ | \ p_k$$. This means that $$gcd(a_i,a_k) \neq 1$$. This is a contradiction since we assumed that $$a_1,...,a_k$$ are pairwise relatively prime. Therefore, we must have $$a_k$$ and $$b$$ be relatively prime. $$\ \blacksquare$$
<br>
<br>
The consequence of this lemma is the following
<br>
<br>
<!------------------------------------------------------------------------>
<div class="peachheaderdiv">
Proposition
</div>
<div class="peachbodydiv">
If \(a_1, a_2,...,a_k\) are pairwise relatively prime and if \(a_i \ | \ n\) for all \(i = 1,...,k\), then \(a_1a_2,...,a_k \ | \ n\) 
</div>
<!------------------------------------------------------------------------>
<br>
<b>Proof</b>
<br>
By Induction on $$k$$ 
<br>
Base Case: If $$k=1$$, then there is nothing to prove. 
<br>
If $$k = 2$$, then $$gcd(a_1,a_2)=1$$. If $$a_1 \ | \ n$$ and $$a_1 \ | \ n$$, then by the proposition from lecture 5, we must have $$ab \ | \ n$$.
<br>
<br>
Inductive Case $$k \geq 3$$: <br>
Let $$b = a_1a_2...a_{k-1}$$.  By the previous lemma we know that $$gcd(a_k,b) = 1$$. Also by the inductive hypothesis if $$a_1,...,a_{k-1} \ | \ n$$, then $$a_1...a_{k-1} = b \ | \ n$$. but $$gcd(a_k,b) = 1$$ so $$a_k$$ and $$b$$ are relatively prime. Since they are relatively prime and they both divide $$n$$, then $$ba_k = a_1...a_{k-1}a_k$$ also divides $$n$$ as we wanted to show. $$\ \blacksquare$$





<hr>

<!------------------------------------------------------------------------>
<h3>References</h3>
<ul>
<li>MATH417 by Charles Rezk</li>
<li><a href="https://homepage.divms.uiowa.edu/~goodman/algebrabook.dir/algebrabook.html">Algebra: Abstract and Concrete by Frederick M. Goodman</a></li>
</ul>






















