---
layout: post
title:  "Euclid Proposition 2"
date:   2024-03-24 07:01:36 -0700
categories: jekyll update
mathjax: true
---
<b>Proposition</b>: Given two triangles $ABC$ and $EDF$. If $BA=DE$, $BC=DF$ and the angle $B$ equals $D$, then $AC=EF$, the angle $A$=$E$ and $C=F$ and both triangles are equal.
<br>
<hr>
<br>
<b>Proof.</b><br>
Suppose
<div center>
$$
\begin{align*}
1 + (-1)^n(2n-1) &= 1 + (-1)^{(2k+1)}(2(2k+1)-1) \\
&= 1 + (-1)^{(2k+1)}(4k+2-1) \\
&= 1 + -1(4k+1) \\
&= 1 + -4k -1 \\
&= -4k.
\end{align*}
$$
</div>
And we see that $-4k$ is a multiple of 4.
<br>
<b>Case 2:</b> Suppose $n$ is even. Then $n = 2k$ for some $k \in Z$ and
<div center>
$$
\begin{align*}
1 + (-1)^n(2n-1) &= 1 + (-1)^{(2k)}(2(2k)-1) \\
&= 1 + (1)(4k-1) \\
&= 1 + 4k - 1 \\
&= 4k.
\end{align*}
$$
</div>
And we see that $4k$ is also a multiple of 4.$\blacksquare$
<br>
<br>
<hr>
<br>
<b>Refererences:</b>
Book of Proof by Richard Hammack.




